TreeItrp.v
@@ -1,10 +1,17 @@
 Require Import List.
 
 Require Import Utils.
-Require Import Context.
-Require Import SimpSubst.
-Require Import SimpSyntax.
+Require Import Substitutions.
 Require Import TreeSyntax.
+Require Import Context.
+Require Import DepItrp.
+
+Import VarBump.
+Import TreeTermBump.
+Import TreeTypes.
+Import TreeVarOKBump.
+
+Set Implicit Arguments.
 
 (* Structured semantic types = type codes = universe construction *)
 
@@ -14,7 +21,7 @@ Inductive TypS : Type->Type :=
 	typUvS : TypS Type |
 	typElS T : TypS T |
 	typPiS A (B:A->Type) : TypS A->(forall a,TypS (B a))->TypS (forall a,B a).
-Implicit Arguments typPiS [A B].
+Arguments typPiS [A B] As Bs.
 
 Example X2s : TypS (forall (X0:Type) (X1:forall (x0:X0),Type),forall (x0:X0) (x1:X1 x0),Type).
 	exact (typPiS typUvS (fun X0=>
@@ -25,106 +32,98 @@ Example X2s : TypS (forall (X0:Type) (X1:forall (x0:X0),Type),forall (x0:X0) (x1
 Qed.
 
 Inductive TypR : Type := typ T (s:TypS T).
-Implicit Arguments typ [T].
 
 Definition Typ := TypR.
 
-Definition typTp (T:Typ) := match T with typ T _ => T end.
-Coercion typTp : Typ >-> Sortclass.
+Definition TypTp (T:Typ) := match T with typ T _ => T end.
+Coercion TypTp : Typ >-> Sortclass.
 
 Definition typSc (T:Typ) : TypS T := match T with typ _ s => s end.
 
-Definition typUv : Typ := typ typUvS.
-Definition typEl T : Typ := typ (typElS T).
-Definition typPi (A:Typ) (B:A->Typ) : Typ := typ (typPiS (typSc A) (fun a=>typSc (B a))).
+Definition TypUv : Typ := typ typUvS.
+Definition TypEl T : Typ := typ (typElS T).
+Definition TypPi (A:Typ) (B:A->Typ) : Typ := typ (typPiS (typSc A) (fun a=>typSc (B a))).
+
+Definition IsTypUv (T:Typ) := match T with
+	typ _ typUvS => True |
+	_ => False
+end.
+
+Definition typUvUnfold T : IsTypUv T->(T = TypUv).
+	destruct T.
+	destruct s;simpl;intro;try solve [destruct H].
+	reflexivity.
+Defined.
+Arguments typUvUnfold [T] H.
 
 Definition IsTypPi (T:Typ) := match T with
 	typ _ (typPiS _ _ _ _) => True |
 	_ => False
 end.
 
-Definition typDom (T:Typ) := match T with
+Definition TypDom (T:Typ) := match T with
 	typ _ (typPiS _ _ A _) => typ A |
 	_ => T
 end.
 
-Definition typCdm T : typDom T->Typ.
+Definition TypCdm T : TypDom T->Typ.
 	destruct T.
-	exact (match s as s return typDom (typ s)->Typ with
+	exact (match s return TypDom (typ s)->Typ with
 		typPiS _ _ _ B => fun a=>typ (B a) |
-		_ => fun _=>typUv
+		_ => fun _=>TypUv
 	end).
 Defined.
 
+Definition typPiUnfold T : IsTypPi T->(T = TypPi (TypDom T) (TypCdm T)).
+	destruct T.
+	destruct s;simpl;intro;try solve [destruct H].
+	reflexivity.
+Defined.
+Arguments typPiUnfold [T] H.
+
 End TypCode.
 
-Module Import CodeContex := Contex TypCode.
+Module Import CodeVarItrpBump := VarItrpBump TypCode.
+Import Contex.
 
 (* Interpretation relations *)
 
 (*
-Inductive SimpParamItrp (G:Ctx) (F:G->Typ) : list nat->forall T:G->Typ,(forall g,F g->T g)->Type :=
-	spItrpNil : SimpParamItrp G F nil F (fun g f=>f) |
-	spItrpCons a la T P (a':AtCtx G a P) B la' :
-		SimpParamItrp G F la (fun g=>typPi (P g) (fun p=>B g p)) la'->
-		SimpParamItrp G F (a :: la) (fun g=>B g (ctxProj a' g)) (fun g f=>la' g f (ctxProj a' g)).
+Inductive TreeTermItrp (G:Ctx) : treeTerm->forall T:G->Typ,(forall g,T g)->Type :=
+	ttItrpVar i T (i':AtCtx G i T) : TreeTermItrp G (var i) T (envProj i') |
+	ttItrpApl f a A B f' a' : TreeTermItrp G f (fun g=>TypPi (A g) (B g)) f'->TreeTermItrp G a A a'->
+		TreeTermItrp G (apl f a) (fun g=>B g (a' g)) (fun g=>f' g (a' g)).
 
-Inductive TreeFamItrp (G:Ctx) : treeFam->(G->Typ)->Type :=
-	tfItrpUv : TreeFamItrp G Uv (fun g=>typUv) |
-	tfItrpEl f la F (f':AtCtx G f F) la' :
-		SimpParamItrp G F la (fun g=>typUv) la'->
-		TreeFamItrp G (El (f,la)) (fun g=>typEl (la' g (ctxProj f' g))) |
-	tfItrpPi A B A' B' : TreeFamItrp G A A'->TreeFamItrp (extCtx G A') B B'->
-		TreeFamItrp G (Pi A B) (fun g=>typPi (A' g) (fun a=>B' (existT A' g a))).
+Inductive TreeTypeItrp (G:Ctx) : treeType->(G->Typ)->Type :=
+	tpItrpUv : TreeTypeItrp G Uv (fun g=>TypUv) |
+	tpItrpEl t t' : TreeTermItrp G t (fun g=>TypUv) t'->TreeTypeItrp G (El t) (fun g=>TypEl (t' g)) |
+	tpItrpPi A B A' B' : TreeTypeItrp G A A'->TreeTypeItrp (ExtCtx G A') B B'->
+		TreeTypeItrp G (Pi A B) (fun g=>TypPi (A' g) (fun a=>B' (existT A' g a))).
 *)
 
-Inductive SPItrpNil (G:Ctx) (F:G->Typ) : forall T:G->Typ,(forall g,F g->T g)->Type :=
-	spItrpNil : SPItrpNil G F F (fun g f=>f).
-Implicit Arguments spItrpNil [G].
+Inductive TTItrpApl (G:Ctx) (Rf Ra:forall T:G->Typ,(forall g,T g)->Type) : forall T:G->Typ,(forall g,T g)->Type :=
+	ttItrpApl A B (Bs:forall g a,TypS (B g a)) f' a' : Rf (fun g=>TypPi (A g) (fun a=>typ (Bs g a))) f'->Ra A a'->
+		TTItrpApl G Rf Ra (fun g=>typ (Bs g (a' g))) (fun g=>f' g (a' g)).
+Arguments ttItrpApl [G Rf Ra A B] Bs [f' a'] Xf Xa.
 
-Inductive SPItrpCons (G:Ctx) (F:G->Typ) a (R:forall T:G->Typ,(forall g,F g->T g)->Type) :
-forall T:G->Typ,(forall g,F g->T g)->Type :=
-	spItrpCons P (a':AtCtx G a P) B (BS:forall g p,TypS (B g p)) la' :
-		R (fun g=>typPi (P g) (fun p=>typ (BS g p))) la'->
-		SPItrpCons G F a R (fun g=>typ (BS g (ctxProj a' g))) (fun g f=>la' g f (ctxProj a' g)).
-Implicit Arguments spItrpCons [G F a R P B la'].
-
-Fixpoint SimpParamItrp G F la : forall T,_->Type := match la with
-	nil => SPItrpNil G F |
-	a :: la => SPItrpCons G F a (SimpParamItrp G F la)
+Fixpoint TreeTermItrp G t := match t with
+	var i => VarItrp G i |
+	apl f a => TTItrpApl G (TreeTermItrp G f) (TreeTermItrp G a)
 end.
 
-Inductive TFItrpEl (G:Ctx) f la : (G->Typ)->Type :=
-	tfItrpEl F (f':AtCtx G f F) la' :
-		SimpParamItrp G F la (fun g=>typUv) la'->
-		TFItrpEl G f la (fun g=>typEl (la' g (ctxProj f' g))).
-Implicit Arguments tfItrpEl [G f la F la'].
+Inductive TPItrpEl (G:Ctx) t : (G->Typ)->Type :=
+	tpItrpEl t' : TreeTermItrp G t (fun g=>TypUv) t'->TPItrpEl G t (fun g=>TypEl (t' g)).
+Arguments tpItrpEl [G t t'] Xt.
 
-Inductive TFItrpPi (G:Ctx) (RA RB:forall G:Ctx,(G->Typ)->Type) : (G->Typ)->Type :=
-	tfItrpPi A' B' (B'S:forall g,TypS (B' g)) : RA G A'->RB (extCtx G A') (fun g=>typ (B'S g))->
-		TFItrpPi G RA RB (fun g=>typPi (A' g) (fun a=>typ (B'S (existT A' g a)))).
-Implicit Arguments tfItrpPi [G RA RB A' B' B'S].
+Inductive TPItrpPi (G:Ctx) (RA RB:forall G:Ctx,(G->Typ)->Type) : (G->Typ)->Type :=
+	tpItrpPi A' B' (B's:forall g,TypS (B' g)) : RA G A'->RB (ExtCtx G A') (fun g=>typ (B's g))->
+		TPItrpPi G RA RB (fun g=>TypPi (A' g) (fun a=>typ (B's (existT A' g a)))).
+Arguments tpItrpPi [G RA RB A' B'] B's XA XB.
 
-Fixpoint TreeFamItrp (G:Ctx) F : (G->Typ)->Type := match F with
-	Uv => eq (fun g=>typUv) |
-	El (f,la) => TFItrpEl G f la |
-	Pi A B => TFItrpPi G (fun G=>TreeFamItrp G A) (fun G=>TreeFamItrp G B)
-end.
-
-(*
-Inductive TreeCtxItrp : list treeFam->Ctx->Type :=
-	tcItrpNil : TreeCtxItrp nil empCtx |
-	tcItrpCons G F G' F' : TreeCtxItrp G G'->TreeFamItrp G' F F'->
-		TreeCtxItrp (F :: G) (extCtx G' F').
-*)
-
-Inductive TCItrpCons R F : Ctx->Type :=
-	tcItrpCons G' F' : R G'->TreeFamItrp G' F F'->TCItrpCons R F (extCtx G' F').
-Implicit Arguments tcItrpCons [R F G' F'].
-
-Fixpoint TreeCtxItrp G : Ctx->Type := match G with
-	nil => eq empCtx |
-	F :: G => TCItrpCons (TreeCtxItrp G) F
+Fixpoint TreeTypeItrp (G:Ctx) T : (G->Typ)->Type := match T with
+	Uv => eq (fun g=>TypUv) |
+	El t => TPItrpEl G t |
+	Pi A B => TPItrpPi G (fun G=>TreeTypeItrp G A) (fun G=>TreeTypeItrp G B)
 end.
 
 Definition sigTEqE A (P:A->Type) (s1 s2:sigT P) : (s1 = s2)->
@@ -132,338 +131,251 @@ Definition sigTEqE A (P:A->Type) (s1 s2:sigT P) : (s1 = s2)->
 	intro.
 	pattern s2.
 	apply (tr _ H).
-	exists (eq_refl _).
+	exists eq_refl.
 	simpl.
 	reflexivity.
 Defined.
-Implicit Arguments sigTEqE [A P s1 s2].
 
 (* Oops *)
 Axiom UIP : forall T (x:T) (p:x = x),eq_refl x = p.
-Implicit Arguments UIP [T x].
 
 Definition projT2Eq A (P:A->Type) a (p1 p2:P a) : (existT P a p1 = existT P a p2)->(p1 = p2).
 	intro.
 	destruct (sigTEqE H).
 	simpl in x,e.
-	revert e.
-	apply (tr (fun x=>tr P x p1 = p2->_) (UIP x)).
-	simpl.
-	exact (fun p=>p).
+	exact (tr (fun x=>tr P x p1 = p2) (eq_sym (UIP x)) e).
 Defined.
-Implicit Arguments projT2Eq [A P a p1 p2].
 
-Lemma spItrpUniq G F la : forall T1 T2 la1 la2,SimpParamItrp G F la T1 la1->SimpParamItrp G F la T2 la2->
-(existT (fun T:G->Typ=>forall g,F g->T g) T1 la1 = existT _ T2 la2).
-	set (Tla (T:G->Typ) := forall g,F g->T g).
-	induction la;simpl;intros.
+Lemma ttItrpUniq G t : forall T1 T2 t1 t2 (X1:TreeTermItrp G t T1 t1) (X2:TreeTermItrp G t T2 t2),
+existT (fun T:G->Typ=>forall g,T g) T1 t1 = existT _ T2 t2.
+	set (Tt (T:G->Typ) := forall g,T g).
+	induction t as [| f ? a ?];simpl;intros.
 
-	destruct H.
-	destruct H0.
-	reflexivity.
+	exact (varItrpUniq X1 X2).
 
-	destruct X as (P1,a1,B1,BS1,la1).
-	destruct X0 as (P2,a2,B2,BS2,la2).
-	simpl in la1,la2.
-	revert B2 BS2 la2 s0.
-	apply (tr (fun xa=>forall B2 (BS2:forall g p,TypS (B2 g p)) la2,
-		SimpParamItrp G F la (fun g=>typPi (xa_T xa g) (fun p=>typ (BS2 g p))) la2->
-		(_ = existT Tla (fun g=>typ (BS2 g (ctxProj (xa_a xa) g)))
-			(fun g f=>la2 g f (ctxProj (xa_a xa) g))))
-	(atCtxUniq a1 a2)).
+	destruct X1 as (A1,B1,Bs1,f1,a1,Xf1,Xa1).
+	destruct X2 as (A2,B2,Bs2,f2,a2,Xf2,Xa2).
+	simpl in f1,f2.
+	revert B2 Bs2 f2 Xf2.
+	apply (tr (fun x:sigT Tt=>forall B2 (Bs2:forall g a,TypS (B2 g a)) f2
+		(Xf2:TreeTermItrp G f (fun g=>TypPi (projT1 x g) (fun a=>typ (Bs2 g a))) f2),
+		_ = existT Tt (fun g=>typ (Bs2 g (projT2 x g))) (fun g=>f2 g (projT2 x g)))
+	(IHt2 _ _ _ _ Xa1 Xa2)).
 	simpl.
-	clear P2 a2.
+	clear IHt2 A2 a2 Xa2.
 	intros.
-	pose proof (IHla _ _ _ _ s X).
-	clear IHla s X.
-	pose (PBla1 := existT Tla (fun g=>typPi (P1 g) (fun p=>typ (BS1 g p))) la1).
-	pose (PBla2 := existT Tla (fun g=>typPi (P1 g) (fun p=>typ (BS2 g p))) la2).
-	change (PBla1 = PBla2) in H.
-	pose (P (s:sigT Tla) g := typTp (typDom (projT1 s g))).
-	pose (BR (s:sigT Tla) g := typCdm (projT1 s g)).
-	change (forall s g,P s g->Typ) in (type of BR).
-	assert {p:P PBla1 = P PBla2 & tr (fun P=>forall g,P g->Typ) p (BR PBla1) = BR PBla2}.
-		rewrite <- H.
-		exists (eq_refl _).
+	pose proof (IHt1 _ _ _ _ Xf1 Xf2).
+	clear IHt1 Xf1 Xf2.
+	pose (ABf1 := existT Tt (fun g=>TypPi (A1 g) (fun a=>typ (Bs1 g a))) f1).
+	pose (ABf2 := existT Tt (fun g=>TypPi (A1 g) (fun a=>typ (Bs2 g a))) f2).
+	change (ABf1 = ABf2) in H.
+	pose (A (s:sigT Tt) g := TypTp (TypDom (projT1 s g))).
+	pose (BR (s:sigT Tt) g := TypCdm (projT1 s g)).
+	change (forall s g,A s g->Typ) in (type of BR).
+	pose (fT (A:G->Type) (BR:forall g,A g->Typ) := forall g a,BR g a).
+	assert (existT (fun A=>sigT (fT A)) (A ABf1) (existT (fT _) (BR ABf1) (projT2 ABf1)) =
+	existT _ (A ABf2) (existT _ (BR ABf2) (projT2 ABf2))).
+		generalize (fun g:G=>I).
+		apply (tr (fun s=>forall H:forall g,IsTypPi (projT1 s g),_ =
+			existT (fun A=>sigT (fT A)) (A s) (existT (fT _) (BR s) (fun g=>tr _ (typPiUnfold (H g)) (projT2 s g))))
+		H).
 		simpl.
+		intros _.
+		change (fun g=>f1 g) with f1.
 		reflexivity.
-	destruct H0 as (PH,BRH).
-	rewrite <- (UIP PH) in BRH.
-	simpl in BRH.
-	clear PH.
-	subst P BR.
-	simpl in BRH.
-	revert la2 PBla2 H.
-	apply (tr (fun X=>forall la2,
-		let PBla2 := existT Tla (fun g=>typPi (P1 g) (fun p=>X g p)) la2 in
-		(PBla1 = PBla2)->
-		(_ = existT Tla (fun g=>X g (ctxProj a1 g)) (fun g f=>la2 g f (ctxProj a1 g))))
-	BRH).
-	unfold Tla at 1.
-	simpl typTp.
-	clear B2 BS2 BRH.
-	intros.
-	rewrite <- (projT2Eq H).
-	reflexivity.
-Qed.
-Implicit Arguments spItrpUniq [G F la T1 T2 la1 la2].
-
-Lemma tfItrpUniq F : forall G F1 F2,TreeFamItrp G F F1->TreeFamItrp G F F2->(F1 = F2).
-	induction F as [| | A ? B ?];[| destruct p as (f,la) |];simpl;intros.
-
-	rewrite <- H.
-	rewrite <- H0.
-	reflexivity.
-
-	destruct X as (F1,f1,la1).
-	destruct X0 as (F2,f2,la2).
-	revert la2 s0.
-	apply (tr (fun xa=>forall la2,SimpParamItrp G (xa_T xa) la (fun g=>typUv) la2->
-		(_ = fun g=>typEl (la2 g (ctxProj (xa_a xa) g)))) (atCtxUniq f1 f2)).
-	simpl.
-	clear F2 f2.
-	intros.
-	pose (el' T la' g :=
-		match T g as Tg return (F1 g->typTp Tg)->Typ with typ _ s =>
-		match s return (F1 g->typTp (typ s))->Typ with
-			typUvS => fun lag=>typEl (lag (ctxProj f1 g)) |
-			_ => fun _=>typUv
-		end end (la' g)).
-	simpl in el'.
-	change ((fun g=>typEl (la1 g (ctxProj f1 g))) = el' (fun g=>typUv) la2).
-	apply (tr (fun Tla=>_ = el' _ (projT2 Tla)) (spItrpUniq s X)).
-	subst el'.
+	clear H.
+	subst ABf1 ABf2 A BR.
+	simpl in H0.
+	pose proof (projT2Eq H0).
+	clear H0.
+	apply (tr (fun x:sigT (fT A1)=>_ = existT Tt (fun g=>projT1 x g (a1 g)) (fun g=>projT2 x g (a1 g))) H).
 	simpl.
 	reflexivity.
-
-	destruct X as (A1,B1,BS1).
-	destruct X0 as (A2,B2,BS2).
-	revert B2 BS2 t2.
-	rewrite <- (IHF1 _ _ _ t t1).
-	clear A2 t1.
-	intros.
-	apply (tr (fun X=>_ = fun g=>typPi (A1 g) (fun a=>X (existT A1 g a))) (IHF2 _ _ _ t0 t2)).
-	reflexivity.
 Qed.
-Implicit Arguments tfItrpUniq [F G F1 F2].
+Arguments ttItrpUniq [G t T1 T2 t1 t2] X1 X2.
 
-Lemma tcItrpUniq G : forall G1 G2,TreeCtxItrp G G1->TreeCtxItrp G G2->(G1 = G2).
-	induction G;simpl;intros.
+Lemma tpItrpUniq T : forall G T1 T2 (X1:TreeTypeItrp G T T1) (X2:TreeTypeItrp G T T2),T1 = T2.
+	induction T as [| | A ? B ?];simpl;intros.
 
-	rewrite <- H.
-	rewrite <- H0.
+	destruct X1.
+	destruct X2.
 	reflexivity.
 
-	destruct X as (G1,F1).
-	destruct X0 as (G2,F2).
-	revert F2 t2.
-	rewrite <- (IHG _ _ t t1).
-	clear G2 t1.
-	intros.
-	rewrite <- (tfItrpUniq t0 t2).
-	reflexivity.
-Qed.
-Implicit Arguments tcItrpUniq [G G1 G2].
-
-Lemma spItrpBump G F n l la GL P (xg:ExtCtx GL l G) : forall T la',SimpParamItrp G F (laBump n l la) T la'->
-SimpParamItrp (ctxBump P xg) (elBump P xg F) (laBump (S n) l la) (elBump P xg T) (elBump P xg la').
-	induction la;simpl.
-
-	intros.
-	destruct H.
-	apply spItrpNil.
-
-	intros.
-	destruct X.
-	pose proof (spItrpCons (atBump P xg a') (elBump P xg BS) (IHla _ _ s)).
-	rewrite <- ctxProj_Bump in X.
-	exact X.
-Qed.
-Implicit Arguments spItrpBump [G F n l la GL T la'].
-
-Lemma spItrpBump_O G F n la T la' P : SimpParamItrp G F (laBump n O la) T la'->
-SimpParamItrp (extCtx G P) (fun g=>F (projT1 g)) (laBump (S n) O la) (fun g=>T (projT1 g)) (fun g=>la' (projT1 g)).
-	apply (spItrpBump P (extOCtx G)).
-Qed.
-Implicit Arguments spItrpBump_O [G F n la T la'].
-
-Lemma tfItrpBump n F GL P : forall G l F' (xg:ExtCtx GL l G),TreeFamItrp G (fBump n l F) F'->
-TreeFamItrp (ctxBump P xg) (fBump (S n) l F) (elBump P xg F').
-	induction F as [| | A ? B ?];[| destruct p as (f,la) |];simpl;intros.
-
-	rewrite <- H.
+	destruct X1 as (t1,X1).
+	destruct X2 as (t2,X2).
+	generalize (fun g:G=>I).
+	apply (tr (fun s:{T:G->Typ & forall g,T g}=>forall H:forall g,IsTypUv (projT1 s g),
+		_ = fun g=>TypEl (tr _ (typUvUnfold (H g)) (projT2 s g))) (ttItrpUniq X1 X2)).
+	simpl.
+	intros _.
 	reflexivity.
 
-	destruct X.
-	pose proof (tfItrpEl (atBump P xg f') (spItrpBump P xg s)).
-	rewrite <- ctxProj_Bump in X.
-	exact X.
-
-	destruct X.
-	apply (tfItrpPi (A' := elBump P xg A')
-	(B'S := fun g=>B'S (existT _ (xc_f' (xcBump P xg) (projT1 g)) (projT2 g)))).
-		exact (IHF1 _ _ _ _ t).
-
-		exact (IHF2 _ _ _ (extSCtx xg A') t0).
+	destruct X1 as (A1,B1,Bs1,XA1,XB1).
+	destruct X2 as (A2,B2,Bs2,XA2,XB2).
+	revert B2 Bs2 XB2.
+	pattern A2.
+	apply (tr _ (IHT1 _ _ _ XA1 XA2)).
+	clear A2 XA2.
+	intros.
+	apply (tr (fun Bf=>_ = fun g=>TypPi (A1 g) (fun a=>Bf (existT A1 g a))) (IHT2 _ _ _ XB1 XB2)).
+	reflexivity.
 Qed.
-Implicit Arguments tfItrpBump [n F GL G l F'].
+Arguments tpItrpUniq [T G T1 T2] X1 X2.
 
-Lemma tfItrpBump_O G n F F' P : TreeFamItrp G (fBump n O F) F'->
-TreeFamItrp (extCtx G P) (fBump (S n) O F) (fun g=>F' (projT1 g)).
-	apply (tfItrpBump P (extOCtx G)).
+Lemma ttItrpBump GL n GL' l G t (X:TeleS GL n GL') (xg:TeleS GL l G) : forall T t' (Xt:TreeTermItrp G t T t'),
+TreeTermItrp (CtxBump X xg) (ttBump n l t) (elBump X xg T) (elBump X xg t').
+	induction t as [| f ? a ?];simpl;intros.
+
+	exact (varItrpBump X xg Xt).
+
+	destruct Xt as (?,?,?,?,?,Xf,Xa).
+	exact (ttItrpApl (elBump X xg Bs) (IHt1 _ _ Xf) (IHt2 _ _ Xa)).
 Qed.
-Implicit Arguments tfItrpBump_O [G n F F'].
+Arguments ttItrpBump [GL n GL' l G t] X xg [T t'] Xt.
 
-Lemma spItrpSubst G F la l b GL P (xg:ExtCtx (extCtx GL P) l G) (b':AtCtx GL b P) : forall T la',
-	SimpParamItrp G F la T la'->
-SimpParamItrp (ctxSubst xg (ctxProj b')) (elSubst xg F (ctxProj b')) (laSubst la l b)
-(elSubst xg T (ctxProj b')) (elSubst xg la' (ctxProj b')).
-	induction la;simpl;intros.
+Lemma tpItrpBump GL n GL' T (X:TeleS GL n GL') : forall l G T' (xg:TeleS GL l G) (XT:TreeTypeItrp G T T'),
+TreeTypeItrp (CtxBump X xg) (tpBump n l T) (elBump X xg T').
+	induction T as [| | A ? B ?];simpl;intros.
 
-	destruct H.
-	apply spItrpNil.
-
-	destruct X.
-	pose proof (spItrpCons (atSubst xg b' a') (elSubst xg BS (ctxProj b')) (IHla _ _ s)).
-	rewrite <- ctxProj_Subst in X.
-	exact X.
-Qed.
-Implicit Arguments spItrpSubst [G F la l b GL P T la'].
-
-Lemma spItrpSubst_O G P F la b T la' (b':AtCtx G b P) : SimpParamItrp (extCtx G P) F la T la'->
-SimpParamItrp G (fun g=>F (existT _ g (ctxProj b' g))) (laSubst la O b) _ (fun g=>la' (existT _ g (ctxProj b' g))).
-	apply (spItrpSubst (extOCtx (extCtx G P)) b').
-Qed.
-Implicit Arguments spItrpSubst_O [G P F la b T la'].
-
-Lemma tfItrpSubst F b GL P (b':AtCtx GL b P) : forall G l F' (xg:ExtCtx (extCtx GL P) l G),TreeFamItrp G F F'->
-TreeFamItrp (ctxSubst xg (ctxProj b')) (fSubst F l b) (elSubst xg F' (ctxProj b')).
-	induction F as [| | A ? B ?];[| destruct p as (f,la) |];simpl;intros.
-
-	rewrite <- H.
+	destruct XT.
 	reflexivity.
 
-	destruct X.
-	pose proof (tfItrpEl (atSubst xg b' f') (spItrpSubst xg b' s)).
-	rewrite <- ctxProj_Subst in X.
-	exact X.
+	destruct XT as (?,Xt).
+	exact (tpItrpEl (ttItrpBump X xg Xt)).
 
-	destruct X.
-	apply (tfItrpPi (A' := elSubst xg A' (ctxProj b'))
-	(B'S := fun g=>B'S (existT _ (xc_f' (xcSubst xg _) (projT1 g)) (projT2 g)))).
-		exact (IHF1 _ _ _ _ t).
+	destruct XT as (?,?,?,XA,XB).
+	apply tpItrpPi with (A' := elBump X xg A') (B' := elBump X (extTeleS xg A') B') (B's := elBump X (extTeleS xg A') B's).
+		exact (IHT1 _ _ _ xg XA).
 
-		exact (IHF2 _ _ _ (extSCtx xg A') t0).
+		exact (IHT2 _ _ _ (extTeleS xg A') XB).
 Qed.
-Implicit Arguments tfItrpSubst [F b GL P G l F'].
+Arguments tpItrpBump [GL n GL' T] X [l G T'] xg XT.
 
-Lemma tfItrpSubst_O G P F b F' (b':AtCtx G b P) : TreeFamItrp (extCtx G P) F F'->
-TreeFamItrp G (fSubst F O b) (fun g=>F' (existT _ g (ctxProj b' g))).
-	apply (tfItrpSubst b' (extOCtx (extCtx G P))).
+Module Import TreeTermItrpBump <: TERMITRPBUMP.
+
+Module CtxTyp := TypCode.
+Module VarItrpBump := CodeVarItrpBump.
+Module TermBump := TreeTermBump.
+Module VarSubst := TreeVarSubst.
+
+Definition TermItrp := TreeTermItrp.
+Definition tmItrpVar G i T t' (Xi:VarItrp G i T t') := Xi.
+Definition tmItrpBump GL n GL' l G t T t' (X:TeleS GL n GL') (xg:TeleS GL l G) : TermItrp G t T t'->_ := ttItrpBump X xg (t' := t').
+
+End TreeTermItrpBump.
+
+Module Import TreeVarItrpSubst := VarItrpSubst TreeTermItrpBump.
+
+Lemma ttItrpSubst GL B l G b b' t (xg:TeleS (ExtCtx GL B) l G) (Xb:TreeTermItrp GL b B b') : forall T t' (Xt:TreeTermItrp G t T t'),
+TreeTermItrp (CtxSubst xg b') (ttSubst l b t) (elSubst xg b' T) (elSubst xg b' t').
+	induction t as [| f ? a ?];simpl;intros.
+
+	exact (varItrpSubst xg Xb Xt).
+
+	destruct Xt as (?,?,?,?,?,Xf,Xa).
+	exact (ttItrpApl (elSubst xg b' Bs) (IHt1 _ _ Xf) (IHt2 _ _ Xa)).
 Qed.
-Implicit Arguments tfItrpSubst_O [G P F b F'].
+Arguments ttItrpSubst [GL B l G b b' t] xg Xb [T t'] Xt.
 
-Lemma tcItrpProj i C : forall G G',(ltd i (length G))->TreeCtxItrp G G'->
-	(forall F,AtCtx G' i F->TreeFamItrp G' (fBump (S i) O (nth i G Uv)) F->C)->
-C.
-	induction i;intros ? ?;(destruct G as [| F];intro;[destruct H |]);simpl;intro;
-	destruct X;intro rtn.
+Lemma tpItrpSubst GL B l G b b' T (xg:TeleS (ExtCtx GL B) l G) (Xb:TreeTermItrp GL b B b') : forall T' (XT:TreeTypeItrp G T T'),
+TreeTypeItrp (CtxSubst xg b') (tpSubst l b T) (elSubst xg b' T').
+	revert l G xg.
+	induction T as [| | A ? B0 ?];simpl;intros.
 
-	apply (rtn _ (topCtx G' F')).
-	apply tfItrpBump_O.
-	rewrite fBump_O.
-	exact t0.
+	destruct XT.
+	reflexivity.
 
-	apply (IHi _ _ H t).
+	destruct XT as (?,Xt).
+	exact (tpItrpEl (ttItrpSubst xg Xb Xt)).
+
+	destruct XT as (?,?,?,XA,XB).
+	apply tpItrpPi with (A' := elSubst xg b' A') (B' := elSubst (extTeleS xg A') b' B') (B's := elSubst (extTeleS xg A') b' B's).
+		exact (IHT1 _ _ xg _ XA).
+
+		exact (IHT2 _ _ (extTeleS xg A') _ XB).
+Qed.
+Arguments tpItrpSubst [GL B l G b b' T] xg Xb [T'] XT.
+
+Module Import TreeTypesItrp <: TYPESITRP.
+
+Module Types := TreeTypes.
+Module VarOKBump := TreeVarOKBump.
+Module TermItrpBump := TreeTermItrpBump.
+
+Definition TypeItrp := TreeTypeItrp.
+
+Definition tyItrpUniq G T T1 T2 : TypeItrp G T T1->TypeItrp G T T2->_ := tpItrpUniq (T2 := T2).
+Definition tyItrpBump GL n GL' l G T T' (X:TeleS GL n GL') : forall xg:TeleS GL l G,TypeItrp G T T'->_ := tpItrpBump X (T' := T').
+Definition tyItrpSubst GL B l G b b' T T' (xg:TeleS _ l G) (Xb:TermItrp GL b B b') : TypeItrp G T T'->_ := tpItrpSubst xg Xb (T' := T').
+
+End TreeTypesItrp.
+
+Module Import TreeContexItrp := ContexItrp TreeTypesItrp.
+
+Inductive ExTreeTermItrp G t T : Type :=
+	exTreeTermItrp T' t' : TreeTermItrp G t T' t'->TreeTypeItrp G T T'->ExTreeTermItrp G t T.
+Arguments exTreeTermItrp [G t T] T' t' Xt XT.
+
+Lemma ttItrpTotal (G:list treeType) (G':Ctx) t T (XG:CtxItrp G G') : TreeTermOK G t T->ExTreeTermItrp G' t T.
+	intro.
+	induction H.
+
+	apply (varItrpTotal XG v).
+	intros ? ? XT Xi.
+	apply (exTreeTermItrp T' (envProj i')) with (1 := Xi) (2 := XT).
+
+	clear H H0.
+	destruct IHTreeTermOK1 as (T,f',Xf).
+	simpl in t.
+	destruct t as (A1,?,?,XA1,XB).
+	simpl in f'.
+	destruct IHTreeTermOK2 as (A2,a',Xa,XA2).
+	revert a' Xa.
+	pattern A2.
+	apply (tr _ (tpItrpUniq XA1 XA2)).
+	clear A2 XA2.
 	intros.
-	apply (rtn _ (popCtx X F')).
-	apply tfItrpBump_O.
-	exact X0.
+	apply (exTreeTermItrp (fun g=>typ (B's (existT A1 g (a' g)))) (fun g=>f' g (a' g))).
+		simpl.
+		exact (ttItrpApl _ Xf Xa).
+
+		exact (tpItrpSubst (empTeleS _) Xa XB).
 Qed.
-Implicit Arguments tcItrpProj [i C G G'].
+Arguments ttItrpTotal [G G' t T] XG _.
 
-Inductive ExSimpParamItrp G F la T : Type :=
-	exSimpParamItrp T' la' : SimpParamItrp G F la T' la'->TreeFamItrp G T T'->ExSimpParamItrp G F la T.
-Implicit Arguments exSimpParamItrp [G F la T].
-
-Lemma tfItrpTotalNest' G F C : TreeFamGood
-	(fun G F la T=>forall G' F',TreeCtxItrp G G'->TreeFamItrp G' F F'->ExSimpParamItrp G' F' la T) G F->
-forall G',TreeCtxItrp G G'->
-	(forall F' (F'S:forall g,TypS (F' g)),TreeFamItrp G' F (fun g=>typ (F'S g))->C)->
+Lemma tpItrpTotal' G T C : TreeTypeOK G T->forall (G':Ctx) (XG:CtxItrp G G'),
+	(forall T' (T's:forall g,TypS (T' g)),TreeTypeItrp G' T (fun g=>typ (T's g))->C)->
 C.
 	intro.
-	induction X;intros ? XG rtn.
+	induction H;intros ? ? rtn.
 
 	apply (rtn _ (fun g=>typUvS)).
 	reflexivity.
 
-	apply (tcItrpProj (lt_ltd l) XG).
-	intros ? f' XF.
-	destruct (p _ _ XG XF) as (?,?,Xla,XU).
-	simpl in XU.
-	revert la' Xla.
-	rewrite <- XU.
-	clear T' XU.
+	destruct (ttItrpTotal XG t0) as (?,?,Xt,XU).
+	revert t' Xt.
+	destruct XU.
 	intros.
-	apply (rtn _ (fun g=>typElS (la' g (ctxProj f' g)))).
-	exact (tfItrpEl f' Xla).
+	apply (rtn _ (fun g=>typElS (t' g))).
+	exact (tpItrpEl Xt).
 
-	clear X1 X2.
-	apply (IHX1 _ XG).
-	intros A' A'S XA.
-	apply (IHX2 (extCtx G' (fun g=>typ (A'S g)))).
-		simpl.
-		exact (tcItrpCons XG XA).
-	intros B' B'S XB.
-	apply (rtn _ (fun g=>typPiS (A'S g) (fun a=>B'S (existT (fun g=>A' g) g a)))).
+	clear H H0.
+	apply (IHTreeTypeOK1 _ XG).
+	intros A' A's XA.
+	apply (IHTreeTypeOK2 (ExtCtx G' (fun g=>typ (A's g))) (ctxItrpCons XG XA)).
+	intros B' B's XB.
+	apply (rtn _ (fun g=>typPiS (A's g) (fun a=>B's (existT A' g a)))).
 	simpl.
-	exact (tfItrpPi XA XB).
+	exact (tpItrpPi _ XA XB).
 Qed.
+Arguments tpItrpTotal' [G T C] _ [G'] XG _.
 
-Lemma tfItrpTotalNest G F C : TreeFamGood
-	(fun G F la T=>forall G' F',TreeCtxItrp G G'->TreeFamItrp G' F F'->ExSimpParamItrp G' F' la T) G F->
-forall G',TreeCtxItrp G G'->
-	(forall F',TreeFamItrp G' F F'->C)->
+Lemma tpItrpTotal G T C : TreeTypeOK G T->forall (G':Ctx) (XG:CtxItrp G G'),
+	(forall T',TreeTypeItrp G' T T'->C)->
 C.
-	intros ? ? XG rtn.
-	apply tfItrpTotalNest' with (1 := X) (2 := XG).
-	intros ? ? XF.
-	exact (rtn _ XF).
+	intros ? ? ? rtn.
+	apply (tpItrpTotal' H XG).
+	intros ? ? XT.
+	exact (rtn _ XT).
 Qed.
-
-Lemma spItrpTotal G F la T : SimpParamGood G F la T->forall G' F',TreeCtxItrp G G'->TreeFamItrp G' F F'->
-ExSimpParamItrp G' F' la T.
-	intro.
-	induction H;intros ? ? XG XF.
-
-	apply (exSimpParamItrp F' (fun g f=>f)).
-		apply spItrpNil.
-
-		exact XF.
-
-	apply (tcItrpProj (lt_ltd H) XG).
-	intros A a' XA.
-	destruct (IHSimpParamGood _ _ XG XF) as (?,?,Xla,XT).
-	simpl in XT.
-	revert la' Xla.
-	destruct XT as (A0,B',B'S,XA0,XB).
-	simpl.
-	revert B' B'S XB.
-	rewrite <- (tfItrpUniq XA XA0).
-	clear A0 XA0.
-	intros.
-	apply (exSimpParamItrp (fun g=>typ (B'S (existT _ g (ctxProj a' g))))
-	(fun g f=>la' g f (ctxProj a' g))).
-		simpl.
-		exact (spItrpCons a' (fun g a=>B'S (existT _ g a)) Xla).
-
-		exact (tfItrpSubst_O _ XB).
-Qed.
-
-Lemma tfItrpTotal G F G' C : TreeFamGoodPG G F->TreeCtxItrp G G'->
-	(forall F',TreeFamItrp G' F F'->C)->
-C.
-	intros ? XG.
-	apply tfItrpTotalNest with (G := G) (2 := XG).
-	exact (tfGoodMap spItrpTotal H).
-Qed.
+Arguments tpItrpTotal [G T C] _ [G'] XG _.
