DepItrp.v
@@ -1,0 +1,228 @@
+Require Import List.
+Require Import Compare_dec.
+
+Require Import Utils.
+Require Import Substitutions.
+Require Import DepTyping.
+Require Import Context.
+
+Require Import Lt.
+
+Set Implicit Arguments.
+
+Module VarItrpBump (Import CtxTyp : CTXTYP).
+
+Module Import Contex := Contex CtxTyp.
+
+Import VarBump.
+
+Definition atBump GL n GL' l G i T (X:TeleS GL n GL') (xg:TeleS GL l G) (a:AtCtx G i T) :
+AtCtx (CtxBump X xg) (varBump n l i) (elBump X xg T).
+	destruct (lt_dec i l) as [Ho | Ho].
+
+	apply (tr (fun v=>AtCtx _ v _) (eq_sym (varBumpLo _ _ _ Ho))).
+	exact (atBumpLo X xg a (lt_ltd Ho)).
+
+	apply (tr (fun v=>AtCtx _ v _) (eq_sym (varBumpHi _ _ _ Ho))).
+	exact (atBumpHi X xg a (not_lt_ltd Ho)).
+Defined.
+Arguments atBump [GL n GL' l G i T] X xg a.
+
+Lemma envProj_Bump GL n GL' l G i T (X:TeleS GL n GL') (xg:TeleS GL l G) (a:AtCtx G i T) :
+elBump X xg (envProj a) = envProj (atBump X xg a).
+	unfold atBump.
+	destruct (lt_dec i l) as [Ho | Ho].
+
+	destruct (eq_sym (varBumpLo n l i Ho)).
+	simpl.
+	apply envProj_BumpLo.
+
+	destruct (eq_sym (varBumpHi n l i Ho)).
+	simpl.
+	apply envProj_BumpHi.
+Qed.
+Arguments envProj_Bump [GL n GL' l G i T] X xg a.
+
+Inductive VarItrp (G:Ctx) i : forall T:G->Typ,(forall g,T g)->Type :=
+	varItrp T (i':AtCtx G i T) : VarItrp G i T (envProj i').
+Arguments varItrp [G i T] i'.
+
+Lemma varItrpUniq G i T1 T2 t1 t2 (X1:VarItrp G i T1 t1) (X2:VarItrp G i T2 t2) :
+existT (fun T:G->Typ=>forall g,T g) T1 t1 = existT _ T2 t2.
+	destruct X1 as (T1,i1).
+	destruct X2 as (T2,i2).
+	apply (tr (fun x=>_ = existT _ (xa_T x) (envProj (xa_a x))) (atCtxUniq i1 i2)).
+	simpl.
+	reflexivity.
+Qed.
+
+Lemma varItrpBump GL n GL' l G i T t' (X:TeleS GL n GL') (xg:TeleS GL l G) (Xi:VarItrp G i T t') :
+VarItrp (CtxBump X xg) (varBump n l i) (elBump X xg T) (elBump X xg t').
+	destruct Xi.
+	apply (tr _ (eq_sym (envProj_Bump X xg i'))).
+	apply varItrp.
+Qed.
+
+End VarItrpBump.
+
+Module Type TERMITRPBUMP.
+
+Declare Module Import CtxTyp : CTXTYP.
+
+Module Import VarItrpBump := VarItrpBump CtxTyp.
+Import Contex.
+
+Declare Module Import TermBump : TERMBUMP.
+
+Module VarSubst := VarSubst TermBump.
+
+Parameter TermItrp : forall (G:Ctx) (t:term) (T:G->Typ) (t':forall g,T g),Type.
+
+Axiom tmItrpVar : forall G i T t',VarItrp G i T t'->TermItrp G (tmVar i) T t'.
+
+Axiom tmItrpBump : forall GL n GL' l G t T t' (X:TeleS GL n GL') (xg:TeleS GL l G),TermItrp G t T t'->
+TermItrp (CtxBump X xg) (tmBump n l t) (elBump X xg T) (elBump X xg t').
+
+End TERMITRPBUMP.
+
+Module VarItrpSubst (Import TermItrpBump : TERMITRPBUMP).
+
+Import CtxTyp VarItrpBump TermBump VarSubst.
+Import Contex.
+
+Lemma varItrpSubst GL B l G b b' i T t' (xg:TeleS (ExtCtx GL B) l G) (Xb:TermItrp GL b B b') (Xi:VarItrp G i T t') :
+TermItrp (CtxSubst xg b') (varSubst l b i) (elSubst xg b' T) (elSubst xg b' t').
+	destruct (lt_eq_lt_dec i l) as [s | Ho];[destruct s as [Ho | Ho] |];pattern (varSubst l b i).
+
+	apply (tr _ (eq_sym (varSubstLt _ _ _ Ho))).
+	apply tmItrpVar.
+	destruct Xi.
+	apply (tr _ (eq_sym (envProj_SubstLt xg b' i' (lt_ltd Ho)))).
+	apply varItrp.
+
+	apply (tr _ (eq_sym (varSubstEq _ _ _ Ho))).
+	assert (Xl := tr (fun i=>VarItrp G i T t') Ho Xi).
+	simpl in Xl.
+	clear i Xi Ho.
+	destruct Xl as (?,l').
+	apply (tr (fun s=>TermItrp _ _ (projT1 s) (projT2 s)) (xcSubstEqUnExt xg b' l')).
+	simpl.
+	set (X := xc_xg' (xcSubst xg b')).
+	change (TeleS GL l (CtxSubst xg b')) in (type of X).
+	exact (tmItrpBump X (empTeleS GL) Xb).
+
+	apply (tr _ (eq_sym (varSubstGt _ _ _ Ho))).
+	apply tmItrpVar.
+	revert Xi.
+	destruct i.
+		destruct (lt_n_O _ Ho).
+	simpl.
+	intro.
+	destruct Xi.
+	apply (tr _ (eq_sym (envProj_SubstGt xg b' i' (lt_ltd Ho)))).
+	apply varItrp.
+Qed.
+
+End VarItrpSubst.
+
+Module Type TYPESITRP.
+
+Declare Module Import Types : TYPES.
+
+Module VarOKBump := VarOKBump Types.
+
+Declare Module Import TermItrpBump : TERMITRPBUMP with Module TermBump := TermBump.
+Import CtxTyp VarItrpBump.Contex.
+
+Parameter TypeItrp : forall (G:Ctx) (T:type) (T':G->Typ),Type.
+
+Axiom tyItrpUniq : forall G T T1 T2,TypeItrp G T T1->TypeItrp G T T2->(T1 = T2).
+
+Axiom tyItrpBump : forall GL n GL' l G T T' (X:TeleS GL n GL') (xg:TeleS GL l G) (XT:TypeItrp G T T'),
+TypeItrp (CtxBump X xg) (tyBump n l T) (elBump X xg T').
+
+Axiom tyItrpSubst : forall GL B l G b b' T T' (xg:TeleS (ExtCtx GL B) l G) (Xb:TermItrp GL b B b') (XT:TypeItrp G T T'),
+TypeItrp (CtxSubst xg b') (tySubst l b T) (elSubst xg b' T').
+
+End TYPESITRP.
+
+Module ContexItrp (Import TypesItrp : TYPESITRP).
+
+Import VarBump.
+
+Import Types VarOKBump TermItrpBump.
+Import CtxTyp VarItrpBump.
+Import Contex.
+
+(*
+Inductive CtxItrp : list type->Ctx->Type :=
+	ctxItrpNil : CtxItrp nil EmpCtx |
+	ctxItrpCons T G G' T' : CtxItrp G G'->TypeItrp G' T T'->
+		CtxItrp (T :: G) (ExtCtx G' T').
+*)
+
+Inductive CtxItrpCons T R : Ctx->Type :=
+	ctxItrpCons G' T' : R G'->TypeItrp G' T T'->CtxItrpCons T R (ExtCtx G' T').
+Arguments ctxItrpCons [T R G' T'] XG XT.
+
+Fixpoint CtxItrp G : Ctx->Type := match G with
+	nil => eq EmpCtx |
+	T :: G => CtxItrpCons T (CtxItrp G)
+end.
+
+Lemma ctxItrpUniq G : forall G1 G2 (X1:CtxItrp G G1) (X2:CtxItrp G G2),G1 = G2.
+	induction G as [| T];simpl;intros.
+
+	destruct X1.
+	destruct X2.
+	reflexivity.
+
+	destruct X1 as (G1,T1,XG1,XT1).
+	destruct X2 as (G2,T2,XG2,XT2).
+	revert T2 XT2.
+	pattern G2.
+	apply (tr _ (IHG _ _ XG1 XG2)).
+	clear G2 XG2.
+	intros.
+	pattern T2.
+	apply (tr _ (tyItrpUniq XT1 XT2)).
+	reflexivity.
+Qed.
+Arguments ctxItrpUniq [G G1 G2] X1 X2.
+
+Lemma ctxItrpProjNoBump i C : forall G G',(ltd i (length G))->CtxItrp G G'->
+	(forall GL T (xg:TeleS GL (S i) G'),AtCtx G' i (fun g=>T (unExt xg g))->TypeItrp GL (nth i G tyDf) T->C)->
+C.
+	induction i;intros ? ?;(destruct G as [| T];intro;[destruct H |]);simpl;intro XG;
+	destruct XG as (?,?,XG,XT);intro rtn.
+
+	exact (rtn _ _ (extTeleS (empTeleS G') T') (topCtx G' T') XT).
+
+	apply (IHi _ _ H XG).
+	intros ? P xg i' XP.
+	exact (rtn _ _ (extTeleS xg T') (popCtx i' T') XP).
+Qed.
+Arguments ctxItrpProjNoBump [i C G G'] _ XG _.
+
+Lemma ctxItrpProj G G' (XG:CtxItrp G G') i C : (ltd i (length G))->
+	(forall T,AtCtx G' i T->TypeItrp G' (tyBump (S i) O (nth i G tyDf)) T->C)->
+C.
+	intros ? rtn.
+	apply (ctxItrpProjNoBump H XG).
+	intros ? ? xg i' XT.
+	exact (rtn _ i' (tyItrpBump xg (empTeleS _) XT)).
+Qed.
+Arguments ctxItrpProj [G G'] XG [i C] _ _.
+
+Lemma varItrpTotal G G' i T (XG:CtxItrp G G') C : VarOK G i T->
+	(forall T' (i':AtCtx G' i T'),TypeItrp G' T T'->VarItrp G' i T' (envProj i')->C)->
+C.
+	intro.
+	destruct H.
+	intro rtn.
+	apply (ctxItrpProj XG (lt_ltd l)).
+	intros ? i' ?.
+	exact (rtn _ _ X (varItrp i')).
+Qed.
+
+End ContexItrp.
