Substitutions.v
@@ -1,0 +1,332 @@
+Require Import Compare_dec.
+
+Require Import Le Lt.
+Require Import Plus.
+
+Module VarBump.
+
+Definition varBump n l i := match nat_compare i l with
+	Lt => i |
+	_ => n + i
+end.
+
+Lemma varBumpLo n l i : (i < l)->(varBump n l i = i).
+	intro.
+	unfold varBump.
+	rewrite (proj1 (nat_compare_lt _ _) H).
+	reflexivity.
+Qed.
+
+Lemma varBumpHi n l i : ~(i < l)->(varBump n l i = n + i).
+	intro.
+	unfold varBump.
+	destruct (nat_compare_spec i l);try reflexivity.
+	exact (match H H0 with end).
+Qed.
+
+Lemma varBump_O l i : varBump O l i = i.
+	unfold varBump.
+	destruct (nat_compare i l);reflexivity.
+Qed.
+
+Lemma varBump_Bump n1 n2 l1 l2 i : (l1 <= l2)->
+(varBump n2 (n1 + l2) (varBump n1 l1 i) = varBump n1 l1 (varBump n2 l2 i)).
+	intro.
+	destruct (lt_dec i l1).
+
+	assert (i < l2).
+		exact (le_trans _ _ _ l H).
+	rewrite varBumpLo with (1 := l).
+	rewrite varBumpLo with (1 := H0).
+	rewrite varBumpLo with (1 := l).
+	apply varBumpLo.
+	apply le_trans with (1 := H0).
+	apply le_plus_r.
+
+	rewrite varBumpHi with (1 := n).
+	destruct (lt_dec i l2).
+		rewrite varBumpLo with (1 := l).
+		rewrite varBumpHi with (1 := n).
+		apply varBumpLo.
+		apply plus_lt_compat_l with (1 := l).
+
+		rewrite varBumpHi with (1 := n0).
+		rewrite varBumpHi;[| intro;apply n0;apply plus_lt_reg_l with (1 := H0)].
+		rewrite varBumpHi;
+		[|
+			intro;
+			apply n;
+			apply le_trans with (2 := H0);
+			apply le_n_S;
+			apply le_plus_r
+		].
+		rewrite plus_assoc.
+		rewrite <- (plus_comm n1).
+		rewrite <- plus_assoc.
+		reflexivity.
+Qed.
+
+Lemma varBumpDiv a b n l i : (n <= b)->(varBump a (l + n) (varBump b l i) = varBump (a + b) l i).
+	intro.
+	destruct (lt_dec i l).
+
+	rewrite varBumpLo with (1 := l0).
+	rewrite varBumpLo with (1 := l0).
+	apply varBumpLo.
+	apply le_trans with (1 := l0).
+	apply le_plus_l.
+
+	rewrite varBumpHi with (1 := n0).
+	rewrite varBumpHi with (1 := n0).
+	rewrite <- plus_assoc.
+	apply varBumpHi.
+	intro.
+	apply n0.
+	apply plus_lt_reg_l with n.
+	rewrite <- (plus_comm l).
+	apply le_trans with (2 := H0).
+	apply le_n_S.
+	apply plus_le_compat_r with (1 := H).
+Qed.
+
+End VarBump.
+
+Module Type TERMBUMP.
+
+Import VarBump.
+
+Parameter term : Type.
+
+Parameter tmVar : forall i:nat,term.
+Parameter tmBump : forall (n l:nat) (t:term),term.
+
+Axiom tmBump_Var : forall n l i,tmBump n l (tmVar i) = tmVar (varBump n l i).
+
+Axiom tmBump_Bump : forall n1 n2 l1 l2 t,(l1 <= l2)->
+(tmBump n2 (n1 + l2) (tmBump n1 l1 t) = tmBump n1 l1 (tmBump n2 l2 t)).
+
+Axiom tmBumpDiv : forall a b n l t,(n <= b)->(tmBump a (l + n) (tmBump b l t) = tmBump (a + b) l t).
+
+End TERMBUMP.
+
+Module VarSubst (Import TermBump : TERMBUMP).
+
+Import VarBump.
+
+Definition varSubst l b i := match nat_compare i l with
+	Lt => tmVar i |
+	Eq => tmBump l O b |
+	Gt => tmVar (pred i)
+end.
+
+Lemma varSubstLt l b i : (i < l)->(varSubst l b i = tmVar i).
+	intro.
+	unfold varSubst.
+	rewrite (proj1 (nat_compare_lt _ _) H).
+	reflexivity.
+Qed.
+
+Lemma varSubstEq l b i : (i = l)->(varSubst l b i = tmBump l O b).
+	intro.
+	unfold varSubst.
+	rewrite (proj2 (nat_compare_eq_iff _ _) H).
+	reflexivity.
+Qed.
+
+Lemma varSubstGt l b i : (i > l)->(varSubst l b i = tmVar (pred i)).
+	intro.
+	unfold varSubst.
+	rewrite (proj1 (nat_compare_gt _ _) H).
+	reflexivity.
+Qed.
+
+Lemma varBump_Subst n x l b i :
+tmBump n (x + l) (varSubst l b i) = varSubst l (tmBump n x b) (varBump n (S x + l) i).
+	destruct (lt_dec i (S x + l)).
+
+	rewrite varBumpLo with (1 := l0).
+	destruct (lt_eq_lt_dec i l);[destruct s |].
+		rewrite varSubstLt with (1 := l1).
+		rewrite varSubstLt with (1 := l1).
+		rewrite tmBump_Var.
+		rewrite varBumpLo;[reflexivity |].
+		apply le_trans with (1 := l1).
+		apply le_plus_r.
+
+		rewrite varSubstEq with (1 := e).
+		rewrite varSubstEq with (1 := e).
+		rewrite <- plus_comm.
+		apply tmBump_Bump.
+		apply le_O_n.
+
+		rewrite varSubstGt with (1 := l1).
+		rewrite varSubstGt with (1 := l1).
+		rewrite tmBump_Var.
+		apply (f_equal tmVar).
+		apply varBumpLo.
+		destruct i.
+			destruct lt_n_O with (1 := l1).
+		simpl in l0 |- *.
+		apply lt_S_n with (1 := l0).
+
+	rewrite varBumpHi with (1 := n0).
+	assert (l < i).
+		apply not_lt.
+		intro.
+		apply n0.
+		apply le_trans with (1 := H).
+		simpl.
+		rewrite plus_n_Sm.
+		apply le_plus_r.
+	rewrite varSubstGt with (1 := H).
+	rewrite tmBump_Var.
+	rewrite varSubstGt;[| apply le_trans with (1 := H);apply le_plus_r].
+	apply (f_equal tmVar).
+	destruct i.
+		destruct lt_n_O with (1 := H).
+	rewrite <- plus_n_Sm.
+	simpl.
+	apply varBumpHi.
+	intro.
+	apply n0.
+	simpl.
+	apply lt_n_S with (1 := H0).
+Qed.
+
+Lemma varSubst_Bump n l1 l2 b i : (l1 <= l2)->
+(varSubst (n + l2) b (varBump n l1 i) = tmBump n l1 (varSubst l2 b i)).
+	intro.
+	destruct (lt_eq_lt_dec i l2);[destruct s |].
+
+	rewrite varSubstLt with (1 := l).
+	rewrite tmBump_Var.
+	destruct (lt_dec i l1).
+		rewrite varBumpLo with (1 := l0).
+		apply varSubstLt.
+		apply le_trans with (1 := l).
+		apply le_plus_r.
+
+		rewrite varBumpHi with (1 := n0).
+		apply varSubstLt.
+		apply plus_lt_compat_l with (1 := l).
+
+	subst i.
+	rewrite varBumpHi with (1 := le_not_lt _ _ H).
+	rewrite varSubstEq with (1 := eq_refl _).
+	rewrite varSubstEq with (1 := eq_refl _).
+	rewrite <- tmBumpDiv with (1 := H).
+	simpl.
+	reflexivity.
+
+	rewrite varBumpHi;[| apply le_not_lt;apply le_trans with (2 := l);apply le_S with (1 := H)].
+	rewrite varSubstGt with (1 := plus_lt_compat_l _ _ _ l).
+	rewrite varSubstGt with (1 := l).
+	rewrite tmBump_Var.
+	apply (f_equal tmVar).
+	destruct i.
+		destruct lt_n_O with (1 := l).
+	rewrite <- plus_n_Sm.
+	simpl.
+	rewrite varBumpHi;[reflexivity |].
+	apply le_not_lt.
+	apply le_trans with (1 := H) (2 := le_S_n _ _ l).
+Qed.
+
+Lemma varSubstDiv n l1 l2 b i : (l1 <= l2 <= l1 + n)->(varSubst l2 b (varBump (S n) l1 i) = tmVar (varBump n l1 i)).
+	intro.
+	destruct H.
+	destruct (lt_dec i l1).
+
+	rewrite varBumpLo with (1 := l).
+	rewrite varBumpLo with (1 := l).
+	apply varSubstLt.
+	apply le_trans with (1 := l) (2 := H).
+
+	rewrite varBumpHi with (1 := n0).
+	rewrite varBumpHi with (1 := n0).
+	apply varSubstGt.
+	simpl.
+	apply le_n_S.
+	apply le_trans with (1 := H0).
+	rewrite <- plus_comm.
+	apply plus_le_compat_l.
+	apply not_lt with (1 := n0).
+Qed.
+
+End VarSubst.
+
+Module Type TERMSUBST.
+
+Declare Module Import TermBump : TERMBUMP.
+
+Module Import VarSubst := VarSubst TermBump.
+
+Parameter tmSubst : forall (l:nat) (b t:term),term.
+
+Axiom tmSubst_Var : forall l b i,tmSubst l b (tmVar i) = varSubst l b i.
+
+Axiom tmSubst_Bump : forall n l1 l2 b t,(l1 <= l2)->
+(tmSubst (n + l2) b (tmBump n l1 t) = tmBump n l1 (tmSubst l2 b t)).
+
+Axiom tmSubstDiv : forall n l1 l2 b t,(l1 <= l2 <= l1 + n)->(tmSubst l2 b (tmBump (S n) l1 t) = tmBump n l1 t).
+
+End TERMSUBST.
+
+Module VarSubstSubst (Import TermSubst : TERMSUBST).
+
+Import TermBump VarSubst.
+
+Lemma varSubst_Subst x l b1 b2 i : tmSubst (x + l) b1 (varSubst l b2 i) =
+tmSubst l (tmSubst x b1 b2) (varSubst (S x + l) b1 i).
+	destruct (lt_eq_lt_dec i (S x + l));[destruct s |].
+
+	rewrite varSubstLt with (1 := l0).
+	rewrite tmSubst_Var.
+	destruct (lt_eq_lt_dec i l);[destruct s |].
+		rewrite varSubstLt with (1 := l1).
+		rewrite varSubstLt with (1 := l1).
+		rewrite tmSubst_Var.
+		apply varSubstLt.
+		apply le_trans with (1 := l1).
+		apply le_plus_r.
+
+		rewrite varSubstEq with (1 := e).
+		rewrite varSubstEq with (1 := e).
+		rewrite <- plus_comm.
+		apply tmSubst_Bump with (1 := le_O_n _).
+
+		rewrite varSubstGt with (1 := l1).
+		rewrite varSubstGt with (1 := l1).
+		rewrite tmSubst_Var.
+		apply varSubstLt.
+		destruct i.
+			destruct lt_n_O with (1 := l1).
+		simpl in l0 |- *.
+		apply lt_S_n with (1 := l0).
+
+	subst i.
+	rewrite varSubstGt with (l := l);[| simpl;apply le_n_S;apply le_plus_r].
+	rewrite tmSubst_Var.
+	rewrite varSubstEq with (1 := eq_refl _).
+	rewrite varSubstEq with (1 := eq_refl _).
+	simpl.
+	rewrite tmSubstDiv;[reflexivity |].
+	simpl.
+	apply conj with (1 := le_O_n _).
+	apply le_plus_r.
+
+	rewrite varSubstGt with (l := l);[| apply le_trans with (2 := l0);apply le_n_S;apply le_plus_r].
+	rewrite varSubstGt with (1 := l0).
+	rewrite tmSubst_Var.
+	rewrite tmSubst_Var.
+	destruct i.
+		destruct lt_n_O with (1 := l0).
+	simpl in l0 |- *.
+	pose proof (lt_S_n _ _ l0).
+	clear l0.
+	rewrite varSubstGt with (1 := H).
+	rewrite varSubstGt with (l := l);[| apply le_trans with (2 := H);apply le_n_S;apply le_plus_r].
+	reflexivity.
+Qed.
+
+End VarSubstSubst.
